# 4.7: Change of Basis

Today, we will learn to move between coordinates in two different bases for the same vector space.

If
$$
B=\{\vec b_1,\vec b_2,\dots,\vec b_n\}
$$
and
$$
C=\{\vec c_1, \vec c_2, \dots,\vec c_n\}
$$
are bases for a vector space $V$, there exists a unique $n\times n$ matrix $P_{C \leftarrow B}$ that changes $B$ coordinates to $C$ coordinates:
$$
[\vec x]_C=P_{C\leftarrow B}[\vec x]_B
$$
for $\vec x$ in $V$.

It’s given by:
$$
P_{C\leftarrow B} = \big[[\vec b_1]_C,\dots,[\vec b_n]_C\big]
$$


**Example** #2:

If $B=\{\vec b_1,\vec b_2\}$ and $C=\{\vec c_1, \vec c_2\}$, where
$$
\vec b_1 = -\vec c_1 + 4\vec c_2
$$
and
$$
\vec b_2 = 5\vec c_1-3\vec c_2
$$
find the change of coordinate matrix from $B$ to $C$. Then, find $[\vec x]_C$ for $\vec x =5\vec b_1+ 3\vec b_2$.



If $\vec b_1 = -\vec c_1 + 4\vec c_2$, then $[\vec b_1]_C=\begin{bmatrix}-1\\4\end{bmatrix}$

If $\vec b_2=5\vec c_1-3\vec c_2$, then $[\vec b_2]_C=\begin{bmatrix}5\\-3\end{bmatrix}$

So,

​	$P_{C\leftarrow B} = \big[[\vec b_1]_C [\vec b_2]_C\big]=\begin{bmatrix}-1&5\\4&-3\end{bmatrix}$





In general, we won’t know $\vec b_1 = -\vec c_1 + 4\vec c_2$

 **Remember**: $P_B = [\vec b_1, \vec b_2, \dots, \vec b_n]$ such that $\vec x = P_B[\vec x]_B$ for $\vec x$ given by standard basis in $\mathbb R^n$.

​	And so, $P_C=[\vec c_1, \dots, \vec c_n]$ then $\vec x = P_C[\vec x]_C$



If $\vec x = P_C[\vec x]_C$, then $P_C^{-1}\vec x=[\vec x]_C$.

​	And if $\vec x = P_B[\vec x]_B$, then $P_C^{-1}P_B[\vec x]_B=[\vec x]_C$ for $P_{C\leftarrow B}=P_C^{-1}P_B$.

​	$[\vec x]_C=P_{C\leftarrow B}[\vec x]_B$

​	

To find ${P_{C\leftarrow B}}$, you set up:

​	$[P_C|P_B]\sim[I|P_{C\leftarrow B}]$





**Example** #8:
$$
B={\begin{bmatrix}-1\\8\end{bmatrix},\begin{bmatrix}1\\-5\end{bmatrix}}\\
C={\begin{bmatrix}1\\4\end{bmatrix},\begin{bmatrix}1\\1\end{bmatrix}}
$$
Find $P_{C\leftarrow B}$.
$$
[P_C~P_B]=\begin{bmatrix}1&1&-1&1\\4&1&8&-5\end{bmatrix}\sim\begin{bmatrix}1&0&3&-2\\0&1&-4&3\end{bmatrix}
$$
Find $P_{B\leftarrow C}$
$$
P_{B\leftarrow C}=P_{C\leftarrow B}^{-1}=\frac1{9-8}\begin{bmatrix}3&2\\4&3\end{bmatrix}=\begin{bmatrix}3&2\\4&3\end{bmatrix}
$$
Also, you could do:

​	$P_C^{-1}P_B$ to find $P_{C\leftarrow B}$.









